backends/hol4/divDefTheory.sig
@@ -4,12 +4,15 @@ sig
   
   (*  Definitions  *)
     val fix_def : thm
+    val fix_exec_def : thm
     val fix_fuel_P_def : thm
     val fix_fuel_def : thm
+    val fix_nexec_def : thm
     val is_valid_fp_body_def : thm
   
   (*  Theorems  *)
     val case_result_switch_eq : thm
+    val fix_exec_fixed_eq : thm
     val fix_fixed_diverges : thm
     val fix_fixed_eq : thm
     val fix_fixed_terminates : thm
@@ -21,6 +24,7 @@ sig
     val fix_fuel_mono_least : thm
     val fix_fuel_not_diverge_eq_fix : thm
     val fix_fuel_not_diverge_eq_fix_aux : thm
+    val fix_nexec_eq_fix : thm
     val fix_not_diverge_implies_fix_fuel : thm
     val fix_not_diverge_implies_fix_fuel_aux : thm
     val is_valid_fp_body_compute : thm
@@ -37,6 +41,10 @@ sig
             fix_fuel ($LEAST (fix_fuel_P f x)) f x
           else Diverge
    
+   [fix_exec_def]  Definition
+      
+      ⊢ fix_exec = fix_nexec 1000000
+   
    [fix_fuel_P_def]  Definition
       
       ⊢ ∀f x n. fix_fuel_P f x n ⇔ ¬is_diverge (fix_fuel n f x)
@@ -45,6 +53,12 @@ sig
       
       ⊢ (∀f x. fix_fuel 0 f x = Diverge) ∧
         ∀n f x. fix_fuel (SUC n) f x = f (fix_fuel n f) x
+   
+   [fix_nexec_def]  Definition
+      
+      ⊢ ∀n f x.
+          fix_nexec n f x =
+          if fix_fuel_P f x n then fix_fuel n f x else fix f x
    
    [is_valid_fp_body_def]  Definition
       
@@ -74,6 +88,10 @@ sig
              | Diverge => Diverge)
         | Fail e => Fail e
         | Diverge => Diverge
+   
+   [fix_exec_fixed_eq]  Theorem
+      
+      ⊢ ∀N f. is_valid_fp_body N f ⇒ ∀x. fix_exec f x = f (fix_exec f) x
    
    [fix_fixed_diverges]  Theorem
       
@@ -150,6 +168,10 @@ sig
           is_valid_fp_body N g ⇒
           ∀n x.
             g (fix_fuel n f) x ≠ Diverge ⇒ g (fix f) x = g (fix_fuel n f) x
+   
+   [fix_nexec_eq_fix]  Theorem
+      
+      ⊢ ∀N f n. is_valid_fp_body N f ⇒ fix_nexec n f = fix f
    
    [fix_not_diverge_implies_fix_fuel]  Theorem
       
